Network_Security_Policy_Verification/TopoS_Helper.thy
@@ -38,4 +38,30 @@ proof -
   with assms show ?thesis by (simp add: some_in_eq)
 qed
 
+
+lemma (in SecurityInvariant_preliminaries) sinvar_valid_remove_minimalize_offending_overapprox:
+  assumes "wf_graph \<lparr>nodes = nodesG, edges = edgesG\<rparr>"
+      and "\<not> sinvar \<lparr>nodes = nodesG, edges = edgesG\<rparr> nP" (*"set_offending_flows \<lparr>nodes = nodesG, edges = edgesG\<rparr> nP \<noteq> {}"*)
+      and "set Es = edgesG" and "distinct Es"
+  shows "sinvar \<lparr>nodes = nodesG, edges = edgesG -
+              set (minimalize_offending_overapprox Es [] \<lparr>nodes = nodesG, edges = edgesG\<rparr> nP) \<rparr> nP"
+proof -
+  from assms have off_Es: "is_offending_flows (set Es) \<lparr>nodes = nodesG, edges = edgesG\<rparr> nP"
+    by (metis (no_types, lifting) Diff_cancel
+        SecurityInvariant_withOffendingFlows.valid_empty_edges_iff_exists_offending_flows defined_offending
+        delete_edges_simp2 graph.select_convs(2) is_offending_flows_def sinvar_monoI) 
+  from minimalize_offending_overapprox_gives_back_an_offending_flow[OF assms(1) off_Es _ assms(4)] have
+    in_offending: "set (minimalize_offending_overapprox Es [] \<lparr>nodes = nodesG, edges = edgesG\<rparr> nP)
+      \<in> set_offending_flows \<lparr>nodes = nodesG, edges = edgesG\<rparr> nP"
+     using assms(3) by simp
+
+  { fix f
+    assume *: "f\<in>set_offending_flows \<lparr>nodes = nodesG, edges = edgesG\<rparr> nP"
+    from * have 1: "sinvar \<lparr>nodes = nodesG, edges = edgesG - f \<rparr> nP"
+      by (metis (hide_lams, mono_tags) SecurityInvariant_withOffendingFlows.valid_without_offending_flows delete_edges_simp2 graph.select_convs(1) graph.select_convs(2))
+    note 1
+  }
+  with in_offending show ?thesis by (simp add: some_in_eq)
+qed
+
 end
